\subsection{}



\subsubsection{}

Suppose first that~$f$ is a split epimorphism.
This means that there exists a morphism~$g \colon y \to x$ with~$f g = \id_y$.
It follows for every object~$c$ of~$\cat{C}$ for the two induced functions
\[
	f_* \colon \cat{C}(c, x) \to \cat{C}(c, y)
	\quad\text{and}\quad
	g_* \colon \cat{C}(c, y) \to \cat{C}(c, x)
\]
that
\[
	(f_* ∘ g_*)(φ)
	=
	f_*( g_*(φ) )
	=
	f_*(g ∘ φ)
	=
	f ∘ g ∘ φ
	=
	\id_y ∘ φ
	=
	φ
\]
for every element~$φ$ of the set~$\cat{C}(c, y)$.
This shows that the function~$g_*$ is right inverse to the function~$f_*$.
The existence of such a right-inverse entails that~$f_*$ is surjective.

Suppose now that the induced function~$f_* \colon \cat{C}(c, x) \to \cat{C}(c, y)$ is surjective for every object~$c$ of~$\cat{C}$.
By choosing~$c$ as~$y$, we can see that the map
\[
	f_*
	\colon
	\cat{C}(y, x) \to \cat{C}(y, y) \,,
	\quad
	g \mapsto f ∘ g
\]
is surjective.
This surjectivity entails that there exists an element~$g$ of~$\cat{C}(y, x)$ -- that is, a morphism~$g$ from~$y$ to~$x$ in~$\cat{C}$ -- such that~$f ∘ g = \id_y$.
The existence of this morphism~$g$ tells us that~$f$ is split epimorphism.



\subsubsection{}

We have the following chain of equivalences:

\begin{align*}
	{}&
	\text{$f \colon x \textto y$ is a split monomorphism in~$\cat{C}$}
	\\
	\iff{}&
	\text{there exists a morphism~$g \colon y \textto x$ in~$\cat{C}$ with~$g f = \id_{x,\cat{C}}$}
	\\
	\iff{}&
	\text{there exists a morphism~$g \colon y \textto x$ in~$\cat{C}$ with~$(g f)^{\op} = \id_{x,\cat{C}}^{\op}$}
	\\
	\iff{}&
	\text{there exists a morphism~$g \colon y \textto x$ in~$\cat{C}$ with~$f^{\op} g^{\op} = \id_{x,\cat{C}^{\op}}$}
	\\
	\iff{}&
	\text{there exists a morphism~$g' \colon x \textto y$ in~$\cat{C}$ with~$f^{\op} g' = \id_{x,\cat{C}^{\op}}$}
	\\
	\iff{}&
	\text{$f^{\op} \colon y \textto x$ is a split epimorphism in~$\cat{C}^{\op}$}
	\\
	\iff{}&
	\text{$f^{\op}_* \colon \cat{C}^{\op}(c, y) \textto \cat{C}^{\op}(c, x)$ is surjective for every object~$c$ of~$\cat{C}^{\op}$}
	\\
	\iff{}&
	\left\{
		\begin{tabular}{@{}l}
			for every object~$c$ of~$\cat{C}^{\op}$ and every morphism~$φ' \colon c \textto x$ in~$\cat{C}^{\op}$ \\
			there exists a morphism~$g' \colon c \textto y$ in~$\cat{C}^{\op}$ with~$φ' = f^{\op} ∘ g'$
		\end{tabular}
	\right.
	\\
	\iff{}&
	\left\{
		\begin{tabular}{@{}l}
			for every object~$c$ of~$\cat{C}$ and every morphism~$φ \colon x \textto c$ in~$\cat{C}$ \\
			there exists a morphism~$g \colon y \textto c$ in~$\cat{C}$ with~$φ^{\op} = f^{\op} ∘ g^{\op}$
		\end{tabular}
	\right.
	\\
	\iff{}&
	\left\{
		\begin{tabular}{@{}l}
			for every object~$c$ of~$\cat{C}$ and every morphism~$φ \colon x \textto c$ in~$\cat{C}$ \\
			there exists a morphism~$g \colon y \textto c$ in~$\cat{C}$ with~$φ^{\op} = (g ∘ f)^{\op}$
		\end{tabular}
	\right.
	\\
	\iff{}&
	\left\{
		\begin{tabular}{@{}l}
			for every object~$c$ of~$\cat{C}$ and every morphism~$φ \colon x \textto c$ in~$\cat{C}$ \\
			there exists a morphism~$g \colon y \textto c$ in~$\cat{C}$ with~$φ = g ∘ f$
		\end{tabular}
	\right.
	\\
	\iff{}&
	\text{$f^* \colon \cat{C}(y, c) \textto \cat{C}(x, c)$ is surjective for every object~$c$ of~$\cat{C}$} \,.
\end{align*}
