\subsection{}

We denote the given isomorphisms by~$φ \colon a \to a'$ and~$ψ \colon b \to b'$.

The commutativities of the four square diagrams are equivalent to the following four equations respectively:
\[
	ψ f φ^{-1} = f' \,,
	\quad
	ψ f = f' φ \,,
	\quad
	f φ^{-1} = ψ^{-1} f' \,,
	\quad
	f = ψ^{-1} f' φ \,.
\]
These four equations are equivalent because~$ψ$ and~$φ$ are isomorphisms:
\[
	\begin{tikzcd}[
			column sep = tiny,
			row sep = huge,
			every arrow/.append style={Rightarrow}
		]
		{}
		&
		ψ f φ^{-1} = f'
		\arrow[shift right]{dl}[above left]{(\ph) ∘ φ}
		\arrow[shift left]{dr}[above right]{ψ^{-1} ∘ (\ph)}
		&
		{}
		\\
		ψ f = f' φ
		\arrow[shift right]{ur}[below right]{(\ph) ∘ φ^{-1}}
		\arrow[shift right]{dr}[below left]{ψ^{-1} ∘ (\ph)}
		&
		{}
		&
		f φ^{-1} = ψ^{-1} f'
		\arrow[shift left]{ul}[below left]{ψ ∘ (\ph)}
		\arrow[shift left]{dl}[below right]{(\ph) ∘ φ}
		\\
		{}
		&
		f = ψ^{-1} f' φ
		\arrow[shift right]{ul}[above right]{ψ ∘ (\ph)}
		\arrow[shift left]{ur}[above left]{(\ph) ∘ φ^{-1}}
		&
		{}
	\end{tikzcd}
\]
I hence suffices to show for one of these four equations that there exists a unique morphism~$f' \colon a' \to b'$ satisfying this equation.
We can use the first equation, as already explained in the textbook.
