\subsection{}

If~$f_* = g_*$, then by considering more specifically~$f_*, g_* \colon \cat{C}(c, c) \to \cat{C}(c, d)$ we find that
\[
	f = f ⋅ \id_c = f_*(\id_c) = g_*(\id_c) = g ⋅ \id_c = g \,.
\]
Similarly, if~$f^* = g^*$, then by considering~$f^*, g^* \colon \cat{C}(d, d) \to \cat{C}(c, d)$ we find that
\[
	f = \id_d ⋅ f = f^*(\id_d) = g^*(\id_d) = \id_d ⋅ g = g \,.
\]
(One could also derive the implication~$f^* = g^* \implies f = g$ from the implication~$f_* = g_* \implies f = g$ via duality.)
