\subsection{}

In the proof of Theorem~3.2.13 we considered the condition
\[
	(F f)(λ_{\dom f}) = λ_{\codom f}
\]
for \emph{every} morphism~$f$ in~$\Set$.
But this condition is trivially satisfied whenever~$f = \id_x$ for some object~$x$, since then
\[
	(F f)(λ_{\dom f})
	=
	(F \id_x)(λ_{\dom \id_x})
	=
	\id_{F x}(λ_x)
	=
	λ_x
	=
	λ_{\codom \id_x}
	=
	λ_{\codom f} \,.
\]
In the product~$∏_{f ∈ \mor \cat{J}} F(\codom f)$ we can therefore leave out all those factors coming from identity morphisms.
